Cleanup

Source/DafnyStandardLibraries/examples/Actions/ActionsExamples.dfy
@@ -38,6 +38,7 @@ module ActionsExamples {
 
     constructor(i: nat)
       ensures this.i == i
+      reads {}
     {
       this.i := i;
     }
@@ -101,7 +102,7 @@ module ActionsExamples {
       requires Requires(t)
       reads Repr
       modifies Modifies(t)
-      decreases Decreases(t).Ordinal()
+      decreases Decreases(t).Ordinal(), 0
       ensures Ensures(t, r)
     {
       assert Requires(t);
@@ -117,114 +118,24 @@ module ActionsExamples {
     }
   }
 
-  method {:rlimit 0} BoxEnumeratorExample() {
+  method BoxEnumeratorExample() {
     var enum: BoxEnumerator := new BoxEnumerator();
     assert |enum.Outputs()| == 0;
     var a := enum.Invoke(());
 
     assert enum.Outputs() == [a];
-    // assert Seq.Map((b: Box) => b.i, enum.Outputs()) == SeqRange(1) == [0];
-    // assert a.i == 0;
-
-    // var b := enum.Invoke(());
-    // var c := enum.Invoke(());
-    // var d := enum.Invoke(());
-    // var e := enum.Invoke(());
   }
 
-  method {:rlimit 0} ConsumerExample() {
+  @IsolateAssertions
+  @ResourceLimit("10e6")
+  method ConsumerExample() {
     var a: DynamicArrayConsumer<nat> := new DynamicArrayConsumer();
     var _ := a.Invoke(1);
     var _ := a.Invoke(2);
     var _ := a.Invoke(3);
     var _ := a.Invoke(4);
     var _ := a.Invoke(5);
-    var _ := a.Invoke(6);
-    assert a.Inputs() == [1, 2, 3, 4, 5, 6];
-    assert a.storage.items == [1, 2, 3, 4, 5, 6];
-  }
-
-  @AssumeCrossModuleTermination
-  class SplitAction extends Action<nat, Producer<nat>>, OutputsFreshProof<nat> {
-
-    ghost predicate Valid()
-      reads this, Repr
-      ensures Valid() ==> this in Repr
-      ensures Valid() ==> ValidHistory(history)
-      decreases height, 0
-    {
-      && this in Repr
-      && ValidHistory(history)
-    }
-
-    constructor ()
-      ensures Valid()
-      ensures fresh(Repr)
-      ensures history == []
-    {
-      history := [];
-      Repr := {this};
-      height := 1;
-    }
-
-    ghost predicate ValidInput(history: seq<(nat, Producer<nat>)>, next: nat)
-      requires ValidHistory(history)
-      decreases height
-    {
-      true
-    }
-    twostate predicate ValidOutput(history: seq<(nat, Producer<nat>)>, nextInput: nat, new nextOutput: Producer<nat>)
-      decreases height
-      ensures ValidOutput(history, nextInput, nextOutput) ==> ValidHistory(history + [(nextInput, nextOutput)])
-    {
-      ValidHistory(history + [(nextInput, nextOutput)]) && fresh(nextOutput)
-    }
-    ghost predicate ValidHistory(history: seq<(nat, Producer<nat>)>)
-      decreases height
-    {
-      true
-    }
-
-    method Invoke(x: nat) returns (result: Producer<nat>)
-      requires Requires(x)
-      reads Repr
-      modifies Modifies(x)
-      decreases Decreases(x).Ordinal()
-      ensures Ensures(x, result)
-    {
-      result := new SeqProducer([x / 2, x - (x / 2)]);
-      UpdateHistory(x, result);
-    }
-
-    ghost function Action(): Action<nat, Validatable> {
-      this
-    }
-
-    twostate lemma ProducedAllNew(input: nat, new output: Validatable)
-      requires old(Action().Valid())
-      requires Action().ValidOutput(old(Action().history), input, output)
-      ensures output.Valid()
-      ensures fresh(output.Repr)
-    {}
-  }
-
-  @IsolateAssertions
-  method ExamplePipeline() {
-    var upstream := new SeqProducer([1, 2, 3, 4, 5]);
-    var mapping := new SplitAction();
-    var processTotalProof := new DefaultTotalActionProof(mapping);
-    assert fresh(upstream.Repr);
-    assert fresh(mapping.Repr);
-    assert fresh(processTotalProof.Repr);
-
-    var mapped := new MappedProducer(upstream, mapping, processTotalProof);
-    var flattened := new FlattenedProducer(mapped, processTotalProof);
-    
-    var collector := new Collector();
-
-    var collectorTotalProof := new DefaultTotalActionProof(collector);
-    flattened.ForEachRemaining(collector, collectorTotalProof);
-    
-    expect collector.values == [0, 1, 1, 1, 1, 2, 2, 2, 2, 3];
+    assert a.Inputs() == [1, 2, 3, 4, 5];
+    assert a.storage.items == [1, 2, 3, 4, 5];
   }
 }
