Source/DafnyStandardLibraries/src/Std/Actions/GenericAction.dfy
@@ -7,28 +7,12 @@ module Std.GenericActions {
 
   import opened Termination
 
-  // A trait to express any imperative action in Dafny.
-  // This is essentially a reflective interface for a method,
-  // with all possible specifications attached.
-  // It can also be thought of as the logical last step
-  // in the progression of arrow types,
-  // from the total, heap-independent ->,
-  // to the partial but still heap-independent -->,
-  // to the heap-reading ~>.
-  // A generic action is thus like a function that can also modify the heap.
   //
-  // (The behavior of a generic action may also be non-deterministic,
-  // but this case seems less useful in practice,
-  // so the definition of a MostlyGenericAction
-  // that may only modify the heap deterministically
-  // is left as an invitation to the sufficiently motivated Dafny contributor!)
+  // A fully general action.
   //
-  // The more specific Action trait can be much more pleasant to use
-  // when composing non-interferring actions together,
-  // such as working with enumerators or streams,
-  // as they make simplifying assumptions that are true for many reusable actions.
-  // However, this more general action may be more flexible
-  // when accepting any kind of callback in a higher-order method.
+  // See https://github.com/dafny-lang/dafny/blob/master/Source/DafnyStandardLibraries/src/Std/Actions/Actions.md
+  // for further details.
+  //
   trait GenericAction<I, O> {
 
     // Specification predicates
